code/experimental/P256/Hacl.Spec.P256.Ladder.fst
@@ -1,0 +1,18 @@
+module Hacl.Spec.P256.Ladder
+
+open Lib.IntTypes
+open Lib.Buffer
+
+open Hacl.Spec.P256.Definitions
+open Hacl.Spec.P256.MontgomeryMultiplication
+
+open FStar.Math.Lemmas
+open Lib.Sequence
+open Lib.ByteSequence
+
+
+type scalar = lbytes 32
+
+let ith_bit (k:scalar) (i:nat{i < 256}) : uint64 =
+	let q = i / 8 in let r = size (i % 8) in
+ 	to_u64 ((index k q >>. r) &. u8 1)
